Remove the move checking in drop statement; added some test cases

rustexamples/test/borrow_test/41.rs
@@ -1,0 +1,13 @@
+
+//rustc +nightly 41.rs -Z polonius=next
+fn main(){
+    let v: i32 = 12;
+    let v1: i32 = 13;
+    let p: &mut i32 = &mut v;
+    let p1: &mut &mut i32 = &mut p;
+    let p2: &mut &mut i32 = &mut *p1;
+    let q: &mut i32 = &mut v1;
+    *p2 = &mut *q;
+    v = 4; // error here
+    **p1 = 13; 
+}
