rustexamples/test/borrow_test/42.rs
@@ -1,0 +1,6 @@
+fn main(){
+    let v: i32 = 1;
+    let x: &mut i32 = &mut v;
+    x = &mut *x;
+    *x = 3;
+}
