rustfrontend/Rusttyping.v
@@ -291,8 +291,8 @@ Inductive wt_pexpr: pexpr -> Prop :=
     wt_pexpr (Econst_long n (Tlong si))
 | wt_Eplace: forall p
     (WTP1: wt_place p)
-    (COPY: is_copyable (typeof_place p) = true)
-    (BYVAL: access_by_value (typeof_place p) = true),
+    (COPY: is_copyable (typeof_place p) = true),
+    (* (BYVAL: access_by_value (typeof_place p) = true), *)
     wt_pexpr (Eplace p (typeof_place p))
 | wt_Ecktag: forall p fid orgs id
     (WTP1: typeof_place p = Tvariant orgs id)
@@ -316,8 +316,8 @@ Inductive wt_pexpr: pexpr -> Prop :=
 Inductive wt_expr: expr -> Prop :=
 | wt_move_place: forall p
     (WT1: wt_place p)
-    (MOVE: is_movable p = true)
-    (BYVAL: access_by_value (typeof_place p) = true),
+    (MOVE: is_movable p = true),
+    (* (BYVAL: access_by_value (typeof_place p) = true), *)
     wt_expr (Emoveplace p (typeof_place p))
 | wt_pure_expr: forall pe
     (SCALAR: scalar_type (typeof_pexpr pe) || is_reference (typeof_pexpr pe) = true)
@@ -326,7 +326,9 @@ Inductive wt_expr: expr -> Prop :=
 .
 
 Definition wt_exprlist al : Prop :=
-  Forall wt_expr al.
+  (* We do not support passing struct/enum via function arguments for
+  now as it would introduce complicated inout parameters mechanism *)
+  Forall (fun e => wt_expr e /\ access_by_value (typeof e) = true) al.
 
 (* We should ensure that in an assignment, when source and target
 types are reference/box/struct/enum, their types must have the same
@@ -799,10 +801,11 @@ Fixpoint type_check_pexpr (pe: pexpr) : res unit :=
       do _ <- type_check_place p;
       if is_copyable (typeof_place p) then
         if type_eq ty (typeof_place p) then
-          if access_by_value (typeof_place p) then
-            OK tt
-          else
-            Error (msg "Eplace type is not accessed by value")
+          OK tt
+          (* if access_by_value (typeof_place p) then *)
+          (*   OK tt *)
+          (* else *)
+          (*   Error (msg "Eplace type is not accessed by value") *)
         else
           Error (msg "Eplace type error")
       else Error (msg "Eplace copying a non-copyable place")
@@ -848,10 +851,11 @@ Definition type_check_expr (e: expr) : res unit :=
       (* else *)
       if is_movable p then
         if type_eq ty (typeof_place p) then
-          if access_by_value (typeof_place p) then
-            OK tt
-          else
-            Error (msg "Emoveplace type is not accessed by value")
+          OK tt
+          (* if access_by_value (typeof_place p) then *)
+          (*   OK tt *)
+          (* else *)
+          (*   Error (msg "Emoveplace type is not accessed by value") *)
         else 
           Error (msg "Emoveplace type error")
       else 
@@ -872,7 +876,10 @@ Fixpoint type_check_exprlist (l: list expr) : res unit :=
   | nil => OK tt
   | e :: l' =>
       do _ <- type_check_expr e;
-      type_check_exprlist l'
+      if access_by_value (typeof e) then
+        type_check_exprlist l'
+      else
+        Error (msg "type_check_exprlist: do not support passing struct/enum as arguments for now")      
   end.
 
 Fixpoint type_check_stmt (stmt: statement) : res unit :=
@@ -1040,10 +1047,10 @@ Proof.
   - monadInv H.
     destruct (is_copyable (typeof_place p)) eqn: COPY; try congruence. 
     destruct type_eq in EQ0; try congruence. subst.
-    destruct (access_by_value (typeof_place p)) eqn: BYVAL; try congruence.
+    (* destruct (access_by_value (typeof_place p)) eqn: BYVAL; try congruence. *)
     econstructor.
     destruct x.
-    eapply type_check_place_sound; eauto. auto. auto.
+    eapply type_check_place_sound; eauto. auto. (* auto. *)
   - destruct (typeof_place p) eqn: TYP; try congruence.
     econstructor; eauto.
     eapply type_check_place_sound; eauto.
@@ -1070,7 +1077,7 @@ Proof.
   - inv H. monadInv H1.    
     destruct is_movable eqn: TYP in EQ0; try congruence.
     destruct type_eq in EQ0; try congruence. subst.
-    destruct (access_by_value (typeof_place p)) eqn: BYVAL; try congruence.
+    (* destruct (access_by_value (typeof_place p)) eqn: BYVAL; try congruence. *)
     destruct x.
     econstructor; eauto.
     eapply type_check_place_sound; eauto.
@@ -1090,8 +1097,10 @@ Proof.
   induction l; simpl; intros.
   econstructor.
   monadInv H. destruct x.
+  destruct (access_by_value (typeof a)) eqn: BYVAL; try congruence.
   econstructor; eauto.
-  eapply type_check_expr_sound; eauto.
+  split.
+  eapply type_check_expr_sound; eauto. auto.
   eapply IHl; eauto.
 Qed.
 
